src/lowparse/LowParse.Spec.VCList.fsti
@@ -699,6 +699,10 @@ let rec refine_nlist_of_nlist_refine_injective
       )
   end
 
+(* This goal used 4.17 of the default rlimit 5 after the switch to per-goal
+   SMT encoding; give it some headroom so it does not flake on slower CI. *)
+#push-options "--z3rlimit 20"
+
 let rec tot_parse_nlist_refine_eq
   (#k: parser_kind)
   (#t: Type)
@@ -741,6 +745,8 @@ let rec tot_parse_nlist_refine_eq
         fl
         b'
   end
+
+#pop-options
 
 let rec nlist_refine_of_refine_nlist
   (#t: Type)
